End of Day 3
- Fixed stepping
- Added is_value
- Added type rule for lambda
- Progress on progress

Lambda.v
@@ -36,15 +36,24 @@ Proof.
   reflexivity.
 Qed.
 
-Definition step (exp : term) : option term :=
+Definition is_value (exp : term) : bool :=
+  match exp with
+  | app _ _ => false
+  | var _   => false
+  | _       => true
+  end.
+
+Fixpoint step (exp : term) : option term :=
   match exp with
   | app t1 t2 => 
-      match t1 with
+      if is_value t1 
+      then match t1 with
       | lambda s _ tm => 
           Some (subst s t2 tm)
       | _ => None
       end
-  | a => Some a 
+      else option_map (fun t1' => app t1' t2) (step t1)
+  | _ => None
   end.
 
 Compute step (app idB (const true)).
@@ -68,23 +77,67 @@ L |- const b : B
  L |- e2 : t1 
 ----------------  [intro_app]
  L |- e1 e2 : t2
+ 
+ (v,t),L |- e : t2 
+-----------------------  [intro_lam]
+ L |- lambda v : t. e : t -> t2
 
 *)
 
+Inductive firstIn (s : string) (t : type) : list (string * type) -> Prop :=
+| fFirst : forall l, firstIn s t (cons (s,t) l) 
+| fDeeper : forall s' t2 l, 
+    s' <> s 
+    -> firstIn s t l
+    -> firstIn s t (cons (s',t2) l) 
+.
+
+
 Inductive typesto : list (string * type) -> term -> type -> Prop :=
-| intro_bool : forall L b, typesto L (const b) B
-| intro_var : forall L v t, In (v, t) L -> typesto L (var v) t
+| intro_bool : forall L b, 
+    typesto L (const b) B
+| intro_var : forall L v t, 
+    firstIn v t L 
+    -> typesto L (var v) t
 | intro_app : forall L e1 e2 t1 t2, 
     typesto L e1 (arr t1 t2)
     -> typesto L e2 t2
     -> typesto L (app e1 e2) t2
+| intro_lam : forall L v e t t2, 
+    typesto (cons (v,t) L) e t2
+    -> typesto L (lambda v t e) (arr t t2)
 .
 
-Theorem progress : forall L e t, typesto L e t -> exists e', step e = Some e'.
+Lemma only_lambda_is_value : forall e L t1 t2 , 
+  is_value e = true 
+  -> typesto L e (arr t1 t2)
+  -> exists s' t' e', e = lambda s' t' e'.
+Proof.
+  intros.
+  inversion H0.
+  - rewrite <- H3 in H.
+    inversion H.
+  - rewrite <- H4 in H. inversion H.
+  - exists v, t1, e0. easy.
+Qed.
+
+Theorem progress : forall L e t, 
+  typesto L e t 
+  -> L = nil
+  -> is_value e = true \/ exists e', step e = Some e'.
 Proof.
   intros.
   induction H.
-  - refine (ex_intro _ (const b) _).
+  - left; reflexivity.
+  - right.
+    rewrite H0 in H.
+    inversion H.
+  - right.
+    apply IHtypesto1 in H0.
+    inversion H0.
+    inversion IHtypesto1.
+  
+  refine (ex_intro _ (const b) _).
     reflexivity.
   - now exists (var v).
   - 
